Add more from the HoTT book to conversion.v

internal/conversion.v
@@ -9,15 +9,14 @@ Local Open Scope string_scope.
 Local Open Scope positive_scope.
 Local Open Scope list_scope.
 
-Definition Context := list Ast.term.
+Definition Context := list (Ast.name * Ast.term).
 Delimit Scope context_scope with ctx.
 Bind Scope context_scope with Context.
-Notation ε := (@nil Ast.term : Context).
-Definition context_extend (Γ : Context) (x : Ast.term) := cons x Γ.
+Notation ε := (@nil (Ast.name * Ast.term) : Context).
+Definition context_extend (Γ : Context) (nx : Ast.name * Ast.term) := cons nx Γ.
 Definition context_app (Γ Γ' : Context) := List.app Γ' Γ.
 Notation "Γ ▻ x" := (context_extend Γ x) (at level 55, right associativity).
 Notation "Γ ▻▻ Γ'" := (context_app Γ Γ') (at level 60, right associativity).
-Print Ast.term.
 
 Definition subst_n_name_def
            (subst_n_name : Ast.term -> Ast.term)
@@ -31,12 +30,16 @@ Definition subst_n_name_def
                Ast.rarg := rarg |}
      end.
 
-Fixpoint subst_n_name (in_term : Ast.term) (subst_term : Ast.term) (var_n : nat) (name : Ast.name) {struct in_term} : Ast.term
+Fixpoint subst_n_name (in_term : Ast.term) (subst_term : Ast.term) (var_n : option nat) (name : Ast.name) {struct in_term} : Ast.term
   := match in_term with
-       | Ast.tRel v => match Compare_dec.lt_eq_lt_dec v var_n with
-                         | inleft (left _) => in_term
-                         | inleft (right _) => subst_term
-                         | inright _ => Ast.tRel (pred v)
+       | Ast.tRel v => match var_n with
+                         | Some var_n'
+                           => match Compare_dec.lt_eq_lt_dec v var_n' with
+                                | inleft (left _) => in_term
+                                | inleft (right _) => subst_term
+                                | inright _ => Ast.tRel (pred v)
+                              end
+                         | None => in_term
                        end
        | Ast.tVar name0 => match name with
                              | Ast.nNamed name1
@@ -61,8 +64,8 @@ Fixpoint subst_n_name (in_term : Ast.term) (subst_term : Ast.term) (var_n : nat)
                               | _, _ => name
                             end in
             Ast.tProd name'
-                      (subst_n_name term0' subst_term (S var_n) new_name)
-                      (subst_n_name term1' subst_term (S var_n) new_name)
+                      (subst_n_name term0' subst_term (option_map S var_n) new_name)
+                      (subst_n_name term1' subst_term (option_map S var_n) new_name)
        | Ast.tLambda name' term0' term1'
          => let new_name := match name, name' with
                               | Ast.nNamed n0, Ast.nNamed n1
@@ -72,8 +75,8 @@ Fixpoint subst_n_name (in_term : Ast.term) (subst_term : Ast.term) (var_n : nat)
                               | _, _ => name
                             end in
             Ast.tLambda name'
-                        (subst_n_name term0' subst_term (S var_n) new_name)
-                        (subst_n_name term1' subst_term (S var_n) new_name)
+                        (subst_n_name term0' subst_term (option_map S var_n) new_name)
+                        (subst_n_name term1' subst_term (option_map S var_n) new_name)
        | Ast.tLetIn name' term0' term1' term2'
          => let new_name := match name, name' with
                               | Ast.nNamed n0, Ast.nNamed n1
@@ -83,9 +86,9 @@ Fixpoint subst_n_name (in_term : Ast.term) (subst_term : Ast.term) (var_n : nat)
                               | _, _ => name
                             end in
             Ast.tLetIn name'
-                       (subst_n_name term0' subst_term (S var_n) new_name)
-                       (subst_n_name term1' subst_term (S var_n) new_name)
-                       (subst_n_name term2' subst_term (S var_n) new_name)
+                       (subst_n_name term0' subst_term (option_map S var_n) new_name)
+                       (subst_n_name term1' subst_term (option_map S var_n) new_name)
+                       (subst_n_name term2' subst_term (option_map S var_n) new_name)
        | Ast.tApp f args
          => Ast.tApp (subst_n_name f subst_term var_n name)
                      (List.map (fun term' => subst_n_name term' subst_term var_n name) args)
@@ -103,19 +106,100 @@ Fixpoint subst_n_name (in_term : Ast.term) (subst_term : Ast.term) (var_n : nat)
        | Ast.tUnknown _ => in_term
      end.
 
-Fixpoint context_subst_n (in_context : Context) (subst_term : Ast.term) (var_n : nat) (name : Ast.name) {struct in_context} : Context
+Fixpoint context_subst_n (in_context : Context) (subst_term : Ast.term) (var_n : option nat) (name : Ast.name) {struct in_context} : Context
   := match in_context with
        | nil => nil
-       | cons T Ts => context_extend
-                        (context_subst_n Ts subst_term (S var_n) name)
-                        (subst_n_name T subst_term var_n name)
+       | cons (n, T) Ts
+         => let name' := match n, name with
+                           | Ast.nNamed n', Ast.nNamed name'
+                             => if string_dec n' name'
+                                then Ast.nAnon
+                                else name
+                           | Ast.nAnon, _ => name
+                           | _, Ast.nAnon => name
+                         end in
+            context_extend
+              (context_subst_n Ts subst_term (option_map S var_n) name')
+              (n, subst_n_name T subst_term var_n name)
      end.
 
 (** Quoting the rules from the appendix of the HoTT book *)
 
-Print Ast.term.
-
 Inductive convertible : Context -> Ast.term -> Ast.term -> Ast.term -> Type :=
+(**
+<<
+  Γ ⊢ a : A
+--------------
+Γ ⊢ a ≡ a :> A
+>> *)
+| conv_refl : forall Γ a A, has_type Γ a A -> convertible Γ a a A
+(**
+<<
+Γ ⊢ a ≡ b :> A
+--------------
+Γ ⊢ b ≡ a :> A
+>> *)
+| conv_sym : forall Γ A a b, convertible Γ a b A -> convertible Γ b a A
+(**
+<<
+Γ ⊢ a ≡ b :> A    Γ ⊢ b ≡ c :> A
+---------------------------------
+         Γ ⊢ a ≡ c :> A
+>> *)
+| conv_trans : forall Γ A a b c, convertible Γ a b A -> convertible Γ b c A -> convertible Γ b c A
+(**
+<<
+Γ ⊢ a ≡ b :> A    Γ ⊢ A ≡ B :> Uᵢ
+---------------------------------
+         Γ ⊢ a ≡ b :> B
+>> *)
+| conv_transfer_type : forall Γ A B a b Ui, convertible Γ a b A -> convertible Γ A B (Ast.tSort Ui) -> convertible Γ a b B
+(**
+<<
+Γ ⊢ A ≡ A' :> Uᵢ    Γ, x : A ⊢ B ≡ B' :> Uᵢ     Γ, x : A ⊢ b ≡ b' :> B
+---------------------------------------------------------------------- Π-intro-eq
+              Γ ⊢ λ x.b ≡ λ x.b' :> Π_(x : A) B
+>> *)
+| conv_pi_intro_eq
+  : forall Γ x A A' B B' b b' Ui,
+      convertible Γ A A' (Ast.tSort Ui)
+      -> convertible (Γ ▻ (x, A)) B B' (Ast.tSort Ui)
+      -> convertible (Γ ▻ (x, A)) b b' B
+      -> convertible Γ (Ast.tLambda x A b) (Ast.tLambda x A b') (Ast.tProd x A B)
+| conv_tApp_empty1 : forall Γ f k T,
+                       convertible Γ f k T
+                       -> convertible Γ (Ast.tApp f []) k T
+| conv_tApp_empty2 : forall Γ f k T,
+                       convertible Γ (Ast.tApp f []) k T
+                       -> convertible Γ f k T
+| conv_tApp_cons1 : forall Γ f x xs k T,
+                       convertible Γ (Ast.tApp (Ast.tApp f [x]) xs) k T
+                       -> convertible Γ (Ast.tApp f (x::xs)) k T
+| conv_tApp_cons2 : forall Γ f x xs k T,
+                      convertible Γ (Ast.tApp f (x::xs)) k T
+                      -> convertible Γ (Ast.tApp (Ast.tApp f [x]) xs) k T
+(**
+<<
+Γ, x : A ⊢ b : B     Γ ⊢ a : A
+---------------------------------------- Π-comp
+Γ ⊢ (λ (x : A). b)(a) ≡ b[a/x] :> B[a/x]
+>> *)
+| conv_beta : forall Γ x A b B a,
+                has_type (Γ ▻ (x, A)) b B
+                -> has_type Γ a A
+                -> convertible Γ (Ast.tApp (Ast.tLambda x A b) [a]) (subst_n_name b a (Some 0%nat) x) (subst_n_name B a (Some 0%nat) x)
+(**
+<<
+Γ ⊢ f : Π_(x : A) B
+---------------------------------------- Π-uniq
+Γ ⊢ f ≡ (λ (x : A). f(x)) :> Π_(x : A) B
+>> *)
+| conv_fun_eta_rel : forall Γ x f A B,
+                       has_type Γ f (Ast.tProd x A B)
+                       -> convertible Γ f (Ast.tLambda x A (Ast.tApp f [Ast.tRel 0])) (Ast.tProd x A B)
+| conv_fun_eta_var : forall Γ x f A B,
+                       has_type Γ f (Ast.tProd (Ast.nNamed x) A B)
+                       -> convertible Γ f (Ast.tLambda (Ast.nNamed x) A (Ast.tApp f [Ast.tVar x])) (Ast.tProd (Ast.nNamed x) A B)
 with has_type : Context -> Ast.term -> Ast.term -> Type :=
 (**
 <<
@@ -123,12 +207,76 @@ with has_type : Context -> Ast.term -> Ast.term -> Type :=
 -------------------------------- Vble
 x₁ : A₁, ..., xₙ : Aₙ ⊢ xᵢ : Aᵢ
 >> *)
-| has_type_tRel_0 : forall T Γ univ,
+| has_type_tRel_0 : forall T Γ n univ,
                       has_type Γ T (Ast.tSort univ)
-                      -> has_type (Γ ▻ T) (Ast.tRel 0) T
+                      -> has_type (Γ ▻ (n, T)) (Ast.tRel 0) T
 | has_type_tRel_S : forall T T' Γ n,
                       has_type Γ (Ast.tRel n) T
-                      -> has_type (Γ ▻ T') (Ast.tRel (S n)) T.
+                      -> has_type (Γ ▻ T') (Ast.tRel (S n)) T
+(**
+<<
+Γ ⊢ a : A     Γ ⊢ A ≡ B :> Uᵢ
+-----------------------------
+        Γ ⊢ a : B
+>> *)
+| has_type_conv_subst
+: forall Γ A a B Ui,
+    has_type Γ a A -> convertible Γ A B (Ast.tSort Ui)
+    -> has_type Γ a B
+(**
+<<
+Γ ctx
+------------ U-intro
+Γ ⊢ Uᵢ : Uᵢ₊₁
+>>
+FIXME: This isn't what the numbers stand for!
+ *)
+| has_type_type
+: forall Γ i, has_type Γ (Ast.tSort (Ast.sType i)) (Ast.tSort (Ast.sType (i+1)))
+(**
+<<
+Γ ⊢ A : Uᵢ
+------------ U-cumul
+Γ ⊢ A : Uᵢ₊₁
+>>
+FIXME: This isn't what the numbers stand for!
+ *)
+| has_type_cumul
+  : forall Γ A i, has_type Γ A (Ast.tSort (Ast.sType i))
+                  -> has_type Γ A (Ast.tSort (Ast.sType (i+1)))
+(**
+<<
+Γ ⊢ A : Uᵢ     Γ, x : A ⊢ B : Uᵢ
+-------------------------------- Π-form
+     Γ ⊢ Π_(x : A) B : Uᵢ
+>> *)
+| has_type_tProd
+  : forall Γ A x Ui B,
+      has_type Γ A (Ast.tSort Ui)
+      -> has_type (Γ ▻ (x, A)) B (Ast.tSort Ui)
+      -> has_type Γ (Ast.tProd x A B) (Ast.tSort Ui)
+(**
+<<
+Γ, x : A ⊢ b : B
+------------------------------- Π-intro
+Γ ⊢ λ (x : A). b : Π_(x : A) B
+>> *)
+| has_type_tLambda
+  : forall Γ x A B b,
+      has_type (Γ ▻ (x, A)) b B
+      -> has_type Γ (Ast.tLambda x A b) (Ast.tProd x A B)
+(**
+<<
+Γ ⊢ f : Π_(x : A) B     Γ ⊢ a : A
+--------------------------------- Π-elim
+Γ ⊢ λ (x : A) ⇒ b : Π_(x : A) B
+>> *)
+| has_type_tApp
+  : forall Γ f x A B a,
+      has_type Γ f (Ast.tProd x A B)
+      -> has_type Γ a A
+      -> has_type Γ (Ast.tApp f [a]) (subst_n_name B a (Some 0%nat) x).
+
 
 Class Context_inf := mkContext : Context.
 Definition Let_Context_inf_In (ctx : Context_inf) {T} (f : Context_inf -> T)
@@ -143,380 +291,66 @@ Definition Let_Context_inf_In (ctx : Context_inf) {T} (f : Context_inf -> T)
 
 HoTT book says provable by induction.
 *)
-Lemma subst_1 {Γ a A Δ B b}
-: has_type Γ a A -> has_type (Γ ▻ A ▻▻ Δ) b B
-  -> has_type (Γ ▻▻ context_subst_n Δ a (List.length Γ) Ast.nAnon)%list
-              (subst_n_name b a (List.length Γ) Ast.nAnon)
-              (subst_n_name B a (List.length Γ) Ast.nAnon).
+Lemma subst_1 {Γ a x A Δ B b}
+: has_type Γ a A -> has_type (Γ ▻ (x, A) ▻▻ Δ) b B
+  -> has_type (Γ ▻▻ context_subst_n Δ a (Some (List.length Γ)) x)%list
+              (subst_n_name b a (Some (List.length Γ)) x)
+              (subst_n_name B a (Some (List.length Γ)) x).
 Proof.
   intros ht1 ht2.
 Admitted.
 
 (**
+<<
+Γ ⊢ A : Uᵢ     Γ, Δ ⊢ b : B
+--------------------------------- Wkg₁
+   Γ, x : A, Δ ⊢ b : B
+>>
 
-
-Local Opaque Compare_dec.lt_eq_lt_dec.
-    simpl in *.
-  simpl.
-  induction ht2
-Γ
-Inductive has_type :  Context -> Ast.term -> Ast.term -> Type :=
-| has_type_weaken : forall Γ Γ' T t,
-                      has_type Γ t T
-                      -> has_type (Γ ++ Γ') t T
-| has_type_tRel_0 : forall T Γ,
-                      has_type (Γ ▻ T) (Ast.tRel 0) T
-| has_type_tRel_S : forall T T' Γ n,
-                      has_type Γ (Ast.tRel n) T
-                      -> has_type (Γ ▻ T') (Ast.tRel (S n)) T
-| has_type_tApp : forall Γ A B f x,
-                    has_type Γ f (A ‘→’ B)
-                    -> has_type Γ x A
-                    -> has_type Γ (Ast.tApp f [x]) B
-| has_type_tApp_nil : forall Γ A x,
-                        has_type Γ x A
-                        -> has_type Γ (Ast.tApp x []) A
-| has_type_tApp_split : forall Γ T f x1 x2 xs,
-                          has_type Γ (Ast.tApp (Ast.tApp f [x1]) (cons x2 xs)) T
-                          -> has_type Γ (Ast.tApp f (cons x1 (cons x2 xs))) T
-(* TODO?: Make sure that the beta-expanded term is well-typed? *)
-| has_type_beta_1_type : forall Γ t f T,
-                           has_type Γ t (f (cbv_beta_1 T))
-                           -> has_type Γ t (f T)
-| has_type_eta_1_type : forall Γ t f T,
-                          has_type Γ t (f T)
-                          -> has_type Γ t (f (cbv_beta_1 T))
-| has_type_beta_1_term : forall Γ f t T,
-                           has_type Γ (f (cbv_beta_1 t)) T
-                           -> has_type Γ (f t) T
-| has_type_eta_1_term : forall Γ t f T,
-                          has_type Γ (f t) T
-                          -> has_type Γ (f (cbv_beta_1 t)) T
-(** TODO?: Make sure that the arguments to [sigT] are well-typed? *)
-| has_type_existT
-  : forall Γ A P x y,
-      (*let T := Ast.tApp ‘sigT’ [A; P] in
-    has_type T (Ast.tSort U)
-    -> has_type A (Ast.tSort U1
-    -> has_type P (A ‘→’ Ast.tSort U2)*)
-      has_type Γ x A
-      -> has_type Γ y (Ast.tApp P [x])
-      -> has_type Γ (Ast.tApp ‘existT’ [A; P; x; y]) (Ast.tApp ‘sigT’ [A; P])
-| has_type_qO : forall Γ, has_type Γ qO nat'
-| has_type_qS : forall Γ, has_type Γ qS (nat' ‘→’ nat')
-| has_type_qxI : forall Γ, has_type Γ qxI (positive' ‘→’ positive')
-| has_type_qxO : forall Γ, has_type Γ qxO (positive' ‘→’ positive')
-| has_type_qxH : forall Γ, has_type Γ qxH positive'
-| has_type_qtrue : forall Γ, has_type Γ qtrue bool'
-| has_type_qfalse : forall Γ, has_type Γ qfalse bool'
-| has_type_qAscii : forall Γ, has_type Γ qAscii (bool' ‘→’ bool' ‘→’ bool' ‘→’ bool' ‘→’ bool' ‘→’ bool' ‘→’ bool' ‘→’ bool' ‘→’ ascii')
-| has_type_qEmptyString : forall Γ, has_type Γ qEmptyString string'
-| has_type_qString : forall Γ, has_type Γ qString (ascii' ‘→’ string' ‘→’ string')
-| has_type_qnil : forall Γ T U, has_type Γ T (Ast.tSort U)
-                              -> has_type Γ (Ast.tApp qnil [T]) (Ast.tApp list' [T])
-| has_type_qcons : forall Γ T,
-                     has_type Γ (Ast.tApp qcons [T]) (T ‘→’ Ast.tApp list' [T] ‘→’ Ast.tApp list' [T])
-| has_type_term' : forall Γ, has_type Γ term' (Ast.tSort Ast.sSet)
-| has_type_def' : forall Γ, has_type Γ def' (Ast.tSort Ast.sSet ‘→’ Ast.tSort Ast.sSet)
-| has_type_qmkInd : forall Γ, has_type Γ qmkInd (string' ‘→’ nat' ‘→’ inductive')
-(*| has_type_qstProp : has_type Γ (qtSort ‘’ qsProp) (Ast.tSort (Ast.sType 1))
-| has_type_qstSet : has_type Γ (qtSort ‘’ qsSet) (Ast.tSort (Ast.sType 1))
-| has_type_qstType : forall p p',
-                      denote_positive p = Some p'
-                      -> has_type Γ (qtSort ‘’ (Ast.tApp qsType [p]))
-                                  (Ast.tSort (Ast.sType (1 + p')))*)
-| has_type_qsProp : forall Γ, has_type Γ qsProp sort'
-| has_type_qsSet : forall Γ, has_type Γ qsSet sort'
-| has_type_qsType : forall Γ, has_type Γ qsType (positive' ‘→’ sort')
-| has_type_qnAnon : forall Γ, has_type Γ qnAnon name'
-| has_type_qnNamed : forall Γ, has_type Γ qnNamed (ident' ‘→’ name')
-| has_type_qVmCast : forall Γ, has_type Γ qVmCast cast_kind'
-| has_type_qNativeCast : forall Γ, has_type Γ qNativeCast cast_kind'
-| has_type_qCast : forall Γ, has_type Γ qCast cast_kind'
-| has_type_qRevertCast : forall Γ, has_type Γ qRevertCast cast_kind'
-| has_type_qtRel : forall Γ, has_type Γ qtRel (nat' ‘→’ term')
-| has_type_qtVar : forall Γ, has_type Γ qtVar (ident' ‘→’ term')
-| has_type_qtMeta : forall Γ, has_type Γ qtMeta (nat' ‘→’ term')
-| has_type_qtEvar : forall Γ, has_type Γ qtEvar (nat' ‘→’ term')
-| has_type_qtSort : forall Γ, has_type Γ qtSort (sort' ‘→’ term')
-| has_type_qtCast : forall Γ, has_type Γ qtCast (term' ‘→’ cast_kind' ‘→’ term' ‘→’ term')
-| has_type_qtProd : forall Γ, has_type Γ qtProd (name' ‘→’ term' ‘→’ term' ‘→’ term')
-| has_type_qtLambda : forall Γ, has_type Γ qtLambda (name' ‘→’ term' ‘→’ term' ‘→’ term')
-| has_type_qtLetIn : forall Γ, has_type Γ qtLetIn (name' ‘→’ term' ‘→’ term' ‘→’ term' ‘→’ term')
-| has_type_qtApp : forall Γ, has_type Γ qtApp (term' ‘→’ Ast.tApp list' [term'] ‘→’ term')
-| has_type_qtConst : forall Γ, has_type Γ qtConst (string' ‘→’ term')
-| has_type_qtInd : forall Γ, has_type Γ qtInd (inductive' ‘→’ term')
-| has_type_qtConstruct : forall Γ, has_type Γ qtConstruct (inductive' ‘→’ nat' ‘→’ term')
-| has_type_qtCase : forall Γ, has_type Γ qtCase (nat' ‘→’ term' ‘→’ term' ‘→’ Ast.tApp list' [term'] ‘→’ term')
-| has_type_qtFix : forall Γ, has_type Γ qtFix (mfixpoint' term' ‘→’ nat' ‘→’ term')
-| has_type_qtUnknown : forall Γ, has_type Γ qtUnknown (string' ‘→’ term')
-| has_type_qmkdef : forall Γ T, has_type Γ qmkdef (name' ‘→’ T ‘→’ T ‘→’ nat' ‘→’ Ast.tApp def' [T])
-| has_type_tLambda
-
-
-Local Notation "x ‘→’ y" := (Ast.tProd Ast.nAnon x y) (at level 99, right associativity, y at level 200).
-
-Fixpoint cbv_beta_1_helper (term : Ast.term) (orig_name : Ast.name) (orig_type : Ast.term) (idx : nat) (subst_in : Ast.term)
-: Ast.term
-  := let cbv_beta_1_helper_helper
-         := (fix cbv_beta_1_helper_helper (xs : list Ast.term) : list Ast.term
-             := match xs with
-                  | nil => nil
-                  | cons x' xs' => cons (cbv_beta_1_helper x' orig_name orig_type idx subst_in) (cbv_beta_1_helper_helper xs')
-                end) in
-     match term with
-       | Ast.tRel idx'
-         => if NPeano.Nat.eq_dec idx idx'
-            then subst_in
-            else term
-       | Ast.tVar _ => term
-       | Ast.tMeta _ => term
-       | Ast.tEvar _ => term
-       | Ast.tSort _ => term
-       | Ast.tCast body cst typ
-         => Ast.tCast (cbv_beta_1_helper body orig_name orig_type idx subst_in) cst (cbv_beta_1_helper typ orig_name orig_type idx subst_in)
-       | Ast.tProd name typ body
-         => Ast.tProd name (cbv_beta_1_helper typ orig_name orig_type idx subst_in) (cbv_beta_1_helper body orig_name orig_type (S idx) subst_in)
-       | Ast.tLambda name typ body
-         => Ast.tLambda name (cbv_beta_1_helper typ orig_name orig_type idx subst_in) (cbv_beta_1_helper body orig_name orig_type (S idx) subst_in)
-       | Ast.tLetIn name typ bodyx body
-         => Ast.tLetIn
-              name
-              (cbv_beta_1_helper typ orig_name orig_type idx subst_in)
-              (cbv_beta_1_helper bodyx orig_name orig_type idx subst_in)
-              (cbv_beta_1_helper body orig_name orig_type (S idx) subst_in)
-       | Ast.tApp f' nil
-         => cbv_beta_1_helper f' orig_name orig_type idx subst_in
-       | Ast.tApp f' args
-         => Ast.tApp (cbv_beta_1_helper f' orig_name orig_type idx subst_in)
-                     (cbv_beta_1_helper_helper args)
-       | Ast.tConst _ => term
-       | Ast.tInd _ => term
-       | Ast.tConstruct _ _ => term
-       | Ast.tCase _ _ _ _
-         => Ast.tApp (Ast.tLambda orig_name orig_type term) [subst_in]
-       | Ast.tFix _ _
-         => Ast.tApp (Ast.tLambda orig_name orig_type term) [subst_in]
-       | Ast.tUnknown _ => term
-     end.
-
-Fixpoint cbv_beta_1 (term : Ast.term) : Ast.term
-  := let cbv_beta_1_helper'
-         := (fix cbv_beta_1_helper' (xs : list Ast.term) : list Ast.term
-             := match xs with
-                  | nil => nil
-                  | cons x' xs' => cons (cbv_beta_1 x') (cbv_beta_1_helper' xs')
-                end) in
-     match term with
-       | Ast.tApp term' nil
-         => term'
-       | Ast.tApp (Ast.tLambda orig_name typ body) (subst_in::xs')
-         => Ast.tApp (cbv_beta_1_helper body orig_name typ 0 subst_in) xs'
-       | Ast.tApp term' ls
-         => Ast.tApp (cbv_beta_1 term') (cbv_beta_1_helper' ls)
-       | Ast.tCast body cst typ
-         => Ast.tCast (cbv_beta_1 body) cst (cbv_beta_1 typ)
-       | Ast.tProd name typ body
-         => Ast.tProd name (cbv_beta_1 typ) (cbv_beta_1 body)
-       | Ast.tLambda name typ body
-         => Ast.tLambda name (cbv_beta_1 typ) (cbv_beta_1 body)
-       | Ast.tLetIn name typ bodyx body
-         => Ast.tLetIn name (cbv_beta_1 typ) (cbv_beta_1 bodyx) (cbv_beta_1 body)
-       | Ast.tConst _ => term
-       | Ast.tInd _ => term
-       | Ast.tConstruct _ _ => term
-       | Ast.tCase _ _ _ _ => term
-       | Ast.tFix _ _ => term
-       | Ast.tUnknown _ => term
-       | Ast.tRel _ | Ast.tVar _ | Ast.tMeta _ | Ast.tEvar _ | Ast.tSort _ => term
-     end.
-
-Inductive has_type :  Context -> Ast.term -> Ast.term -> Type :=
-| has_type_weaken : forall Γ Γ' T t,
-                      has_type Γ t T
-                      -> has_type (Γ ++ Γ') t T
-| has_type_tRel_0 : forall T Γ,
-                      has_type (Γ ▻ T) (Ast.tRel 0) T
-| has_type_tRel_S : forall T T' Γ n,
-                      has_type Γ (Ast.tRel n) T
-                      -> has_type (Γ ▻ T') (Ast.tRel (S n)) T
-| has_type_tApp : forall Γ A B f x,
-                    has_type Γ f (A ‘→’ B)
-                    -> has_type Γ x A
-                    -> has_type Γ (Ast.tApp f [x]) B
-| has_type_tApp_nil : forall Γ A x,
-                        has_type Γ x A
-                        -> has_type Γ (Ast.tApp x []) A
-| has_type_tApp_split : forall Γ T f x1 x2 xs,
-                          has_type Γ (Ast.tApp (Ast.tApp f [x1]) (cons x2 xs)) T
-                          -> has_type Γ (Ast.tApp f (cons x1 (cons x2 xs))) T
-(* TODO?: Make sure that the beta-expanded term is well-typed? *)
-| has_type_beta_1_type : forall Γ t f T,
-                           has_type Γ t (f (cbv_beta_1 T))
-                           -> has_type Γ t (f T)
-| has_type_eta_1_type : forall Γ t f T,
-                          has_type Γ t (f T)
-                          -> has_type Γ t (f (cbv_beta_1 T))
-| has_type_beta_1_term : forall Γ f t T,
-                           has_type Γ (f (cbv_beta_1 t)) T
-                           -> has_type Γ (f t) T
-| has_type_eta_1_term : forall Γ t f T,
-                          has_type Γ (f t) T
-                          -> has_type Γ (f (cbv_beta_1 t)) T
-(** TODO?: Make sure that the arguments to [sigT] are well-typed? *)
-| has_type_existT
-  : forall Γ A P x y,
-      (*let T := Ast.tApp ‘sigT’ [A; P] in
-    has_type T (Ast.tSort U)
-    -> has_type A (Ast.tSort U1
-    -> has_type P (A ‘→’ Ast.tSort U2)*)
-      has_type Γ x A
-      -> has_type Γ y (Ast.tApp P [x])
-      -> has_type Γ (Ast.tApp ‘existT’ [A; P; x; y]) (Ast.tApp ‘sigT’ [A; P])
-| has_type_qO : forall Γ, has_type Γ qO nat'
-| has_type_qS : forall Γ, has_type Γ qS (nat' ‘→’ nat')
-| has_type_qxI : forall Γ, has_type Γ qxI (positive' ‘→’ positive')
-| has_type_qxO : forall Γ, has_type Γ qxO (positive' ‘→’ positive')
-| has_type_qxH : forall Γ, has_type Γ qxH positive'
-| has_type_qtrue : forall Γ, has_type Γ qtrue bool'
-| has_type_qfalse : forall Γ, has_type Γ qfalse bool'
-| has_type_qAscii : forall Γ, has_type Γ qAscii (bool' ‘→’ bool' ‘→’ bool' ‘→’ bool' ‘→’ bool' ‘→’ bool' ‘→’ bool' ‘→’ bool' ‘→’ ascii')
-| has_type_qEmptyString : forall Γ, has_type Γ qEmptyString string'
-| has_type_qString : forall Γ, has_type Γ qString (ascii' ‘→’ string' ‘→’ string')
-| has_type_qnil : forall Γ T U, has_type Γ T (Ast.tSort U)
-                              -> has_type Γ (Ast.tApp qnil [T]) (Ast.tApp list' [T])
-| has_type_qcons : forall Γ T,
-                     has_type Γ (Ast.tApp qcons [T]) (T ‘→’ Ast.tApp list' [T] ‘→’ Ast.tApp list' [T])
-| has_type_term' : forall Γ, has_type Γ term' (Ast.tSort Ast.sSet)
-| has_type_def' : forall Γ, has_type Γ def' (Ast.tSort Ast.sSet ‘→’ Ast.tSort Ast.sSet)
-| has_type_qmkInd : forall Γ, has_type Γ qmkInd (string' ‘→’ nat' ‘→’ inductive')
-(*| has_type_qstProp : has_type Γ (qtSort ‘’ qsProp) (Ast.tSort (Ast.sType 1))
-| has_type_qstSet : has_type Γ (qtSort ‘’ qsSet) (Ast.tSort (Ast.sType 1))
-| has_type_qstType : forall p p',
-                      denote_positive p = Some p'
-                      -> has_type Γ (qtSort ‘’ (Ast.tApp qsType [p]))
-                                  (Ast.tSort (Ast.sType (1 + p')))*)
-| has_type_qsProp : forall Γ, has_type Γ qsProp sort'
-| has_type_qsSet : forall Γ, has_type Γ qsSet sort'
-| has_type_qsType : forall Γ, has_type Γ qsType (positive' ‘→’ sort')
-| has_type_qnAnon : forall Γ, has_type Γ qnAnon name'
-| has_type_qnNamed : forall Γ, has_type Γ qnNamed (ident' ‘→’ name')
-| has_type_qVmCast : forall Γ, has_type Γ qVmCast cast_kind'
-| has_type_qNativeCast : forall Γ, has_type Γ qNativeCast cast_kind'
-| has_type_qCast : forall Γ, has_type Γ qCast cast_kind'
-| has_type_qRevertCast : forall Γ, has_type Γ qRevertCast cast_kind'
-| has_type_qtRel : forall Γ, has_type Γ qtRel (nat' ‘→’ term')
-| has_type_qtVar : forall Γ, has_type Γ qtVar (ident' ‘→’ term')
-| has_type_qtMeta : forall Γ, has_type Γ qtMeta (nat' ‘→’ term')
-| has_type_qtEvar : forall Γ, has_type Γ qtEvar (nat' ‘→’ term')
-| has_type_qtSort : forall Γ, has_type Γ qtSort (sort' ‘→’ term')
-| has_type_qtCast : forall Γ, has_type Γ qtCast (term' ‘→’ cast_kind' ‘→’ term' ‘→’ term')
-| has_type_qtProd : forall Γ, has_type Γ qtProd (name' ‘→’ term' ‘→’ term' ‘→’ term')
-| has_type_qtLambda : forall Γ, has_type Γ qtLambda (name' ‘→’ term' ‘→’ term' ‘→’ term')
-| has_type_qtLetIn : forall Γ, has_type Γ qtLetIn (name' ‘→’ term' ‘→’ term' ‘→’ term' ‘→’ term')
-| has_type_qtApp : forall Γ, has_type Γ qtApp (term' ‘→’ Ast.tApp list' [term'] ‘→’ term')
-| has_type_qtConst : forall Γ, has_type Γ qtConst (string' ‘→’ term')
-| has_type_qtInd : forall Γ, has_type Γ qtInd (inductive' ‘→’ term')
-| has_type_qtConstruct : forall Γ, has_type Γ qtConstruct (inductive' ‘→’ nat' ‘→’ term')
-| has_type_qtCase : forall Γ, has_type Γ qtCase (nat' ‘→’ term' ‘→’ term' ‘→’ Ast.tApp list' [term'] ‘→’ term')
-| has_type_qtFix : forall Γ, has_type Γ qtFix (mfixpoint' term' ‘→’ nat' ‘→’ term')
-| has_type_qtUnknown : forall Γ, has_type Γ qtUnknown (string' ‘→’ term')
-| has_type_qmkdef : forall Γ T, has_type Γ qmkdef (name' ‘→’ T ‘→’ T ‘→’ nat' ‘→’ Ast.tApp def' [T])
-| has_type_tLambda
-  : forall Γ name name' A B body,
-      has_type (A::Γ) body B
-      -> has_type Γ (Ast.tLambda name A body) (Ast.tProd name' A B).
-
-Existing Class has_type.
-Existing Instances
-         has_type_tApp has_type_tApp_nil has_type_tApp_split
-         has_type_qO has_type_qS
-         has_type_qtRel has_type_qtVar has_type_qtMeta has_type_qtEvar has_type_qtSort has_type_qtCast has_type_qtProd has_type_qtLambda has_type_qtLetIn has_type_qtApp has_type_qtConst has_type_qtInd has_type_qtConstruct has_type_qtCase has_type_qtFix has_type_qtUnknown
-         has_type_qtrue has_type_qfalse
-         has_type_qAscii
-         has_type_qEmptyString has_type_qString
-         has_type_qxI has_type_qxO has_type_qxH
-         has_type_qnil has_type_qcons
-         has_type_qsProp has_type_qsSet has_type_qsType
-         has_type_qnAnon has_type_qnNamed
-         has_type_qVmCast has_type_qNativeCast has_type_qCast has_type_qRevertCast
-         has_type_qmkInd has_type_qmkdef
-         has_type_term' has_type_def'
-         has_type_tRel_S has_type_tRel_0.
-
-Instance quote_nat_has_type {Γ} (n : nat)
-: has_type Γ (quote n) nat'.
-Proof. induction n; simpl; exact _. Defined.
-
-Instance quote_bool_has_type {Γ} (x : bool)
-: has_type Γ (quote x) bool'.
-Proof. destruct x; simpl; exact _. Defined.
-
-Instance quote_ascii_has_type {Γ} (x : Ascii.ascii)
-: has_type Γ (quote x) ascii'.
-Proof. destruct x; simpl; try exact _. Defined.
-
-Instance quote_string_has_type {Γ} (x : string)
-: has_type Γ (quote x) string'.
-Proof. induction x; simpl; try exact _. Defined.
-
-Instance quote_ident_has_type {Γ} (x : Ast.ident)
-: has_type Γ (quote x) string'
-  := quote_string_has_type x.
-
-Instance quote_positive_has_type {Γ} (x : positive)
-: has_type Γ (quote x) positive'.
-Proof. induction x; simpl; try exact _. Defined.
-
-Instance quote_list_has_type {Γ T T' U}
-         `{Quotable T, has_type Γ T' (Ast.tSort U), forall a : T, has_type Γ (quote a) T'}
-         (x : list T)
-: has_type Γ (quote_list T' x) (Ast.tApp list' [T']).
-Proof. unfold quote; induction x; simpl; try exact _. Defined.
-
-Instance quote_inductive_has_type {Γ} (x : Ast.inductive)
-: has_type Γ (quote x) inductive'.
-Proof. unfold quote; destruct x; simpl; try exact _. Defined.
-
-Instance quote_sort_has_type {Γ} (x : Ast.sort)
-: has_type Γ (quote x) sort'.
-Proof. unfold quote; destruct x; try exact _. Defined.
-
-Instance quote_name_has_type {Γ} (x : Ast.name)
-: has_type Γ (quote x) name'.
-Proof. unfold quote; destruct x; simpl; try exact _. Defined.
-
-Instance quote_cast_kind_has_type {Γ} (x : Ast.cast_kind)
-: has_type Γ (quote x) cast_kind'.
-Proof. unfold quote; destruct x; simpl; try exact _. Defined.
-
-Local Arguments quote_term_step : simpl never.
-
-Fixpoint quote_term_has_type {Γ} (x : Ast.term)
-: has_type Γ (quote x) term'.
+HoTT book says provable by induction.  But we actually need to bump [Rel], eeeeew
+*)
+(*Lemma wkg_1 {Γ x A Δ B b Ui}
+: has_type Γ A (Ast.tSort Ui) -> has_type (Γ ▻▻ Δ) b B
+  -> has_type (Γ ▻ (x, A) ▻▻ Δ) b B.
 Proof.
-  destruct x; try (unfold quote; simpl; exact _).
-  { unfold quote, term_quotable; simpl.
-    unfold quote_term_step; simpl.
-    repeat apply has_type_tApp_split.
-    eapply has_type_tApp; try exact _; [].
-    let ls := match goal with ls : list Ast.term |- _ => constr:ls end in
-    induction ls; try exact _. }
-  { unfold quote, term_quotable; simpl.
-    unfold quote_term_step; simpl.
-    repeat apply has_type_tApp_split.
-    eapply has_type_tApp; try exact _; [].
-    let ls := match goal with ls : list Ast.term |- _ => constr:ls end in
-    induction ls; try exact _. }
-  { unfold quote, term_quotable; simpl; unfold quote_term_step; simpl.
-    destruct m as [ | [ ] ]; simpl; try exact _; [].
-    repeat apply has_type_tApp_split.
-    eapply has_type_tApp; try exact _; [].
-    repeat apply has_type_tApp_split.
-    eapply has_type_tApp; try exact _; [].
-    repeat apply has_type_tApp_split.
-    eapply has_type_tApp; try exact _; [].
-    clear -quote_term_has_type.
-    let ls := match goal with ls : list (Ast.def Ast.term) |- _ => constr:ls end in
-    induction ls as [ | [ ] ]; simpl; try exact _. }
-Defined.
+Admitted.*)
+
+(**
+<<
+Γ ⊢ a : A     Γ, x : A, Δ ⊢ b ≡ c :> B
+-------------------------------------- Subst₂
+   Γ, Δ[a/x] ⊢ b[a/x] ≡ c[a/x] :> B[a/x]
+>>
+
+HoTT book says provable by induction.
+*)
+Lemma subst_2 {Γ x a A Δ B b c}
+: has_type Γ a A -> convertible (Γ ▻ (x, A) ▻▻ Δ) b c B
+  -> convertible (Γ ▻▻ context_subst_n Δ a (Some (List.length Γ)) x)%list
+                 (subst_n_name b a (Some (List.length Γ)) x)
+                 (subst_n_name c a (Some (List.length Γ)) x)
+                 (subst_n_name B a (Some (List.length Γ)) x).
+Proof.
+  intros ht1 conv1.
+Admitted.
+
+(**
+<<
+Γ ⊢ A : Uᵢ     Γ, Δ ⊢ b ≡ c :> B
+--------------------------------- Wkg₁
+   Γ, x : A, Δ ⊢ b ≡ c :> B
+>>
+
+HoTT book says provable by induction.  But we actually need to bump [Rel], eeeewww
+*)
+(*Lemma wkg_2 {Γ A Δ B b c Ui}
+: has_type Γ A (Ast.tSort Ui) -> convertible (Γ ▻▻ Δ) b c B
+  -> convertible (Γ ▻ A ▻▻ Δ) b c B.
+Proof.
+Admitted.*)
+
+Definition is_a_type Γ (T : Ast.term)
+  := { Ui : _ & has_type Γ T (Ast.tSort Ui) }.
+Lemma is_a_type_good {Γ t T} : has_type Γ t T -> is_a_type Γ T.
+Proof.
+Admitted.
